x86/AsmFacts.v
@@ -241,3 +241,47 @@ Proof.
     intro. eapply Mem.support_return_frame_1 in Heqo2. apply Heqo2.
     eapply Mem.sup_include_pop_stage; eauto.
 Qed.
+
+  Section WITH_SAEQ.
+
+    Variable (ge tge: Genv.t Asm.fundef unit).
+    Hypothesis (SADDR_EQ: forall id ofs, Genv.symbol_address ge id ofs = Genv.symbol_address tge id ofs).
+
+(*    Lemma eval_ros_same: forall ros rs,
+        eval_ros tge ros rs = eval_ros ge ros rs.
+    Proof.
+      unfold eval_ros. intros.
+      destruct ros; auto.
+    Qed.
+*)
+    Lemma eval_addrmode32_same: forall a rs,
+        eval_addrmode32 ge a rs = eval_addrmode32 tge a rs.
+    Proof.
+      intros. unfold eval_addrmode32.
+      destruct a. destruct base, ofs, const; auto.
+      - destruct p, p0; congruence.
+      - destruct p; congruence.
+      - destruct p, p0; congruence.
+      - destruct p; congruence.
+    Qed.
+
+    Lemma eval_addrmode64_same: forall a rs,
+        eval_addrmode64 ge a rs = eval_addrmode64 tge a rs.
+    Proof.
+      intros. unfold eval_addrmode64.
+      destruct a. destruct base, ofs, const; auto.
+      - destruct p, p0; congruence.
+      - destruct p; congruence.
+      - destruct p, p0; congruence.
+      - destruct p; congruence.
+    Qed.
+
+    Lemma eval_addrmode_same: forall a rs,
+        eval_addrmode ge a rs = eval_addrmode tge a rs.
+    Proof.
+      intros. unfold eval_addrmode. destruct Archi.ptr64.
+      - eapply eval_addrmode64_same; eauto.
+      - eapply eval_addrmode32_same; eauto.
+    Qed.
+
+    End WITH_SAEQ.
